Unified_PW_Hashing.thy
@@ -1,0 +1,203 @@
+theory Unified_PW_Hashing
+  imports Worklist_Subsumption_PW_Multiset DRAT_Misc
+begin
+
+subsection \<open>Towards an Implementation\<close>
+locale Worklist1_Defs = Search_Space_Defs +
+  fixes succs :: "'a \<Rightarrow> 'a list"
+begin
+
+definition "add_pw_unified_spec passed wait a \<equiv> SPEC (\<lambda>(passed',wait',brk).
+  if \<exists> x \<in> set (succs a). F x then brk
+  else passed' \<subseteq> passed \<union> {x \<in> set (succs a). \<not> (\<exists> y \<in> passed. x \<preceq> y)}
+      \<and> passed \<subseteq> passed'
+      \<and> wait \<subseteq># wait'
+      \<and> wait' \<subseteq># wait + mset ([x \<leftarrow> succs a. \<not> (\<exists> y \<in> passed. x \<preceq> y)])
+      \<and> (\<forall> x \<in> set (succs a). \<exists> y \<in> passed'. x \<preceq> y)
+      \<and> (\<forall> x \<in> set (succs a). \<not> (\<exists> y \<in> passed. x \<preceq> y) \<longrightarrow> (\<exists> y \<in># wait'. x \<preceq> y))
+      \<and> \<not> brk)
+"
+
+definition "add_pw passed wait a \<equiv>
+    nfoldli (succs a) (\<lambda>(_, _, brk). \<not>brk)
+      (\<lambda>a (passed, wait, brk). RETURN (
+        if F a then
+          (passed, wait, True)
+        else if \<exists> x \<in> passed. a \<preceq> x then
+          (passed, wait, False)
+        else (insert a passed, add_mset a wait, False)
+      ))
+      (passed, wait, False)
+"
+
+end -- \<open>Worklist1 Defs\<close>
+
+locale Worklist1 = Worklist1_Defs + Search_Space +
+  assumes succs_correct: "reachable a \<Longrightarrow> set (succs a) = Collect (E a)"
+begin
+
+lemma add_pw_unified_spec_ref:
+  "add_pw_unified_spec passed wait a \<le> add_pw_spec passed wait a"
+  if "reachable a" "a \<in> passed"
+  using succs_correct[OF that(1)] that(2)
+  unfolding add_pw_unified_spec_def add_pw_spec_def
+  apply simp
+  apply safe
+                      apply (auto simp: empty_subsumes)
+  using mset_subset_eqD apply force
+    using mset_subset_eqD apply force
+  subgoal premises prems
+    using prems (1,6,7,11)
+    by (subst (asm) filter_False; fastforce intro: trans)
+      (* s/h *)
+proof -
+  fix aa :: "'a set" and aaa :: "'a multiset" and b :: bool and x :: 'a
+  assume a1: "\<forall>x\<in>aa. \<exists>xa\<in>passed. x \<preceq> xa"
+  assume a2: "x \<in> aa"
+  assume a3: "aa \<subseteq> passed \<union> {x. E a x \<and> (\<forall>xa\<in>passed. \<not> x \<preceq> xa)}"
+  obtain aab :: "'a \<Rightarrow> 'a" where
+    "\<forall>a. a \<notin> aa \<or> aab a \<in> passed \<and> a \<preceq> aab a"
+    using a1 by moura
+  then show "x \<in> passed"
+    using a3 a2 by blast
+qed
+  (* by (smt UnE mem_Collect_eq subsetCE) *)
+
+
+lemma add_pw_ref:
+  "add_pw passed wait a \<le> \<Down> Id (add_pw_unified_spec passed wait a)"
+  unfolding add_pw_def add_pw_unified_spec_def
+  apply (refine_vcg
+      nfoldli_rule[where I =
+        "\<lambda> l1 l2 (passed', wait', brk).
+        if brk then \<exists> a' \<in> set (succs a). F a'
+        else passed' \<subseteq> passed \<union> {x \<in> set l1. \<not> (\<exists> y \<in> passed. x \<preceq> y)}
+           \<and> passed  \<subseteq> passed'
+           \<and> wait \<subseteq># wait'
+           \<and> wait' \<subseteq># wait + mset [x \<leftarrow> l1. \<not> (\<exists> y \<in> passed. x \<preceq> y)]
+           \<and> (\<forall> x \<in> set l1. \<exists> y \<in> passed'. x \<preceq> y)
+           \<and> (\<forall> x \<in> set l1. \<not> (\<exists> y \<in> passed. x \<preceq> y) \<longrightarrow> (\<exists> y \<in># wait'. x \<preceq> y))
+           \<and> set l1 \<inter> Collect F = {}
+      "
+        ])
+     apply (auto; fail)
+    apply (clarsimp split: if_split_asm)
+     apply safe[]
+           apply (auto simp add: subset_mset.le_iff_add; fail)+
+  subgoal premises prems
+    using prems(4,9,11,12,14) by (blast intro: trans)
+  by (auto simp: subset_mset.le_iff_add)
+
+end -- \<open>Worklist 1\<close>
+
+locale Worklist2_Defs = Worklist1_Defs + Search_Space''_Defs
+begin
+
+definition "add_pw' passed wait a \<equiv>
+    nfoldli (succs a) (\<lambda>(_, _, brk). \<not>brk)
+      (\<lambda>a (passed, wait, brk). RETURN (
+        if F a then
+          (passed, wait, True)
+        else if empty a then
+          (passed, wait, False)
+        else if \<exists> x \<in> passed. a \<unlhd> x then
+          (passed, wait, False)
+        else (insert a passed, add_mset a wait, False)
+      ))
+      (passed, wait, False)
+"
+
+definition pw_algo_unified where
+    "pw_algo_unified = do
+      {
+        if F a\<^sub>0 then RETURN True
+        else do {
+          (passed, wait) \<leftarrow> RETURN ({a\<^sub>0}, {#a\<^sub>0#});
+          (passed, wait, brk) \<leftarrow> WHILEIT pw_inv (\<lambda> (passed, wait, brk). \<not> brk \<and> wait \<noteq> {#})
+            (\<lambda> (passed, wait, brk). do
+              {
+                (a, wait) \<leftarrow> take_from_mset wait;
+                ASSERT (reachable a);
+                add_pw' passed wait a
+              }
+            )
+            (passed, wait, False);
+            RETURN brk
+        }
+      }
+    "
+
+end -- \<open>Worklist 2 Defs\<close>
+
+locale Worklist2 = Worklist2_Defs + Worklist1 + Search_Space''_pre + Search_Space
+begin
+
+lemma empty_subsumes'2:
+  "empty x \<or> x \<unlhd> y \<longleftrightarrow> x \<preceq> y"
+  using empty_subsumes' empty_subsumes by auto
+
+lemma bex_or:
+  "P \<or> (\<exists> x \<in> S. Q x) \<longleftrightarrow> (\<exists> x \<in> S. P \<or> Q x)" if "S \<noteq> {}"
+  using that by auto
+
+lemma add_pw'_ref':
+  "add_pw' passed wait a \<le> \<Down> (Id \<inter> {((p, w, _), _). p \<noteq> {} \<and> set_mset w \<subseteq> p}) (add_pw passed wait a)"
+  if "passed \<noteq> {}" "set_mset wait \<subseteq> passed"
+  unfolding add_pw'_def add_pw_def
+  apply (rule nfoldli_refine)
+     apply refine_dref_type
+  using that apply (auto; fail)+
+  apply refine_rcg
+  apply rule
+  unfolding z3_rule(44)
+   apply (subst bex_or)
+  by (auto simp add: empty_subsumes'2)
+
+(* XXX Why is transitivity reasoning broken here? *)
+lemma add_pw'_ref1[refine]:
+  "add_pw' passed wait a \<le> \<Down> (Id \<inter> {((p, w, _), _). p \<noteq> {} \<and> set_mset w \<subseteq> p}) (add_pw_spec passed' wait' a')"
+  if "passed \<noteq> {}" "set_mset wait \<subseteq> passed" "reachable a" "a \<in> passed"
+     and [simp]: "passed = passed'" "wait = wait'" "a = a'"
+proof -
+  from add_pw_unified_spec_ref[OF that(3-4), of wait] add_pw_ref[of passed wait a] have
+    "add_pw passed wait a \<le> \<Down> Id (add_pw_spec passed wait a)"
+    by simp
+  moreover note add_pw'_ref'[OF that(1,2), of a]
+  ultimately show ?thesis
+    by (auto simp add: pw_le_iff refine_pw_simps)
+qed
+
+lemma refine_weaken:
+  "p \<le> \<Down> R p'" if "p \<le> \<Down> S p'" "S \<subseteq> R"
+  using that
+  by (auto simp: pw_le_iff refine_pw_simps; blast)
+
+lemma add_pw'_ref:
+  (* "add_pw' passed wait a \<le> \<Down> (Id \<inter> {((p, w, _), _). p \<noteq> {} \<and> set_mset w \<subseteq> p}) (add_pw_spec passed' wait' a')" *)
+  "add_pw' passed wait a \<le> \<Down> ({((p, w, b), (p', w', b')). p \<noteq> {} \<and> p = p' \<union> set_mset w \<and> w = w' \<and> b = b'}) (add_pw_spec passed' wait' a')"
+  if "passed \<noteq> {}" "set_mset wait \<subseteq> passed" "reachable a" "a \<in> passed"
+     and [simp]: "passed = passed'" "wait = wait'" "a = a'"
+  by (rule add_pw'_ref1[OF that, THEN refine_weaken]; auto)
+
+lemma
+  "(({a\<^sub>0}, {#a\<^sub>0#}, False), {}, {#a\<^sub>0#}, False) \<in> {((p, w, b), (p', w', b')). p = p' \<union> set_mset w' \<and> w = w' \<and> b = b'}"
+  by auto
+
+lemma [refine]:
+  "RETURN ({a\<^sub>0}, {#a\<^sub>0#}) \<le> \<Down> (Id \<inter> {((p, w), (p', w')). p \<noteq> {} \<and> set_mset w \<subseteq> p}) init_pw_spec"
+  unfolding init_pw_spec_def by (auto simp: pw_le_iff refine_pw_simps)
+
+lemma [refine]:
+  "take_from_mset wait \<le> \<Down> {((x, wait), (y, wait')). x = y \<and> wait = wait' \<and> set_mset wait \<subseteq> passed \<and> x \<in> passed} (take_from_mset wait')"
+  if "wait = wait'" "set_mset wait \<subseteq> passed" "wait \<noteq> {#}"
+  using that
+  by (auto 4 5 simp: pw_le_iff refine_pw_simps dest: in_diffD dest!: take_from_mset_correct)
+
+lemma pw_algo_unified_ref:
+  "pw_algo_unified \<le> \<Down> Id pw_algo"
+  unfolding pw_algo_unified_def pw_algo_def
+  by refine_rcg (auto simp: init_pw_spec_def)
+
+end -- \<open>Worklist 2\<close>
+
+end -- \<open>End of Theory\<close>
